\def \equationFirst {y'' + y' - 4y = 0}

\def \equationSecond {y'' - 2y' + 10y = 5x^2 \cdot e^x \cdot \cos{3x}}

\def \equationThird {x^2 \cdot (2\ln{x} - 1) \cdot y'' + 4y = x \cdot (2\ln{x} + 1) \cdot y'}

\def \equationFourth {x(y'' - y)\sin{x} + 2(xy' + y)\cos{x} + 2y'\sin{x} = e^x}

\def \equationFifth {(x^2 + 1)y'' = 2y}

\newcommand{\solutionItemFirst}[3]{
    \item 
    	$ #1 $
    	
    \begin{tabular}[t]{l p{10.6cm}}
    	\textit{Характеристика:} & #2 \\
    	\textit{Общее решение:} & $ #3 $ \\
    \end{tabular}
}
